add a general gmap_auth library and use it where possible

theories/base_logic/lib/wsat.v
@@ -1,6 +1,6 @@
 From stdpp Require Export coPset.
 From iris.proofmode Require Import tactics.
-From iris.algebra Require Import gmap auth agree gset coPset.
+From iris.algebra Require Import gmap_auth gset coPset.
 From iris.base_logic.lib Require Export own.
 From iris Require Import options.
 
@@ -9,7 +9,7 @@ exception of what's in the [invG] module. The module [invG] is thus exported in
 [fancy_updates], which [wsat] is only imported. *)
 Module invG.
   Class invG (Σ : gFunctors) : Set := WsatG {
-    inv_inG :> inG Σ (authR (gmapUR positive (agreeR (laterO (iPropO Σ)))));
+    inv_inG :> inG Σ (gmap_authR positive (laterO (iPropO Σ)));
     enabled_inG :> inG Σ coPset_disjR;
     disabled_inG :> inG Σ (gset_disjR positive);
     invariant_name : gname;
@@ -18,12 +18,12 @@ Module invG.
   }.
 
   Definition invΣ : gFunctors :=
-    #[GFunctor (authRF (gmapURF positive (agreeRF (laterOF idOF))));
+    #[GFunctor (gmap_authRF positive (laterOF idOF));
       GFunctor coPset_disjUR;
       GFunctor (gset_disjUR positive)].
 
   Class invPreG (Σ : gFunctors) : Set := WsatPreG {
-    inv_inPreG :> inG Σ (authR (gmapUR positive (agreeR (laterO (iPropO Σ)))));
+    inv_inPreG :> inG Σ (gmap_authR positive (laterO (iPropO Σ)));
     enabled_inPreG :> inG Σ coPset_disjR;
     disabled_inPreG :> inG Σ (gset_disjR positive);
   }.
@@ -33,10 +33,10 @@ Module invG.
 End invG.
 Import invG.
 
-Definition invariant_unfold {Σ} (P : iProp Σ) : agree (later (iProp Σ)) :=
-  to_agree (Next P).
+Definition invariant_unfold {Σ} (P : iProp Σ) : later (iProp Σ) :=
+  Next P.
 Definition ownI `{!invG Σ} (i : positive) (P : iProp Σ) : iProp Σ :=
-  own invariant_name (◯ {[ i := invariant_unfold P ]}).
+  own invariant_name (gmap_auth_frag_ro i (invariant_unfold P)).
 Arguments ownI {_ _} _ _%I.
 Typeclasses Opaque ownI.
 Instance: Params (@invariant_unfold) 1 := {}.
@@ -54,7 +54,7 @@ Instance: Params (@ownD) 3 := {}.
 
 Definition wsat `{!invG Σ} : iProp Σ :=
   locked (∃ I : gmap positive (iProp Σ),
-    own invariant_name (● (invariant_unfold <$> I : gmap _ _)) ∗
+    own invariant_name (gmap_auth_auth_ro (invariant_unfold <$> I)) ∗
     [∗ map] i ↦ Q ∈ I, ▷ Q ∗ ownD {[i]} ∨ ownE {[i]})%I.
 
 Section wsat.
@@ -106,22 +106,15 @@ Lemma ownD_singleton_twice i : ownD {[i]} ∗ ownD {[i]} ⊢ False.
 Proof. rewrite ownD_disjoint. iIntros (?); set_solver. Qed.
 
 Lemma invariant_lookup (I : gmap positive (iProp Σ)) i P :
-  own invariant_name (● (invariant_unfold <$> I : gmap _ _)) ∗
-  own invariant_name (◯ {[i := invariant_unfold P]}) ⊢
+  own invariant_name (gmap_auth_auth_ro (invariant_unfold <$> I)) ∗
+  own invariant_name (gmap_auth_frag_ro i (invariant_unfold P)) ⊢
   ∃ Q, ⌜I !! i = Some Q⌝ ∗ ▷ (Q ≡ P).
 Proof.
-  rewrite -own_op own_valid auth_both_validI /=. iIntros "[#HI #HvI]".
-  iDestruct "HI" as (I') "HI". rewrite gmap_equivI gmap_validI.
-  iSpecialize ("HI" $! i). iSpecialize ("HvI" $! i).
-  rewrite lookup_fmap lookup_op lookup_singleton option_equivI.
-  case: (I !! i)=> [Q|] /=; [|case: (I' !! i)=> [Q'|] /=; by iExFalso].
-  iExists Q; iSplit; first done.
-  iAssert (invariant_unfold Q ≡ invariant_unfold P)%I as "?".
-  { case: (I' !! i)=> [Q'|] //=.
-    iRewrite "HI" in "HvI". rewrite uPred.option_validI agree_validI.
-    iRewrite -"HvI" in "HI". by rewrite agree_idemp. }
-  rewrite /invariant_unfold.
-  by rewrite agree_equivI later_equivI.
+  rewrite -own_op own_valid gmap_auth_auth_ro_frag_ro_validI.
+  rewrite lookup_fmap option_equivI.
+  case: (I !! i)=> [Q|] /=; last by eauto.
+  iIntros "?". iExists Q; iSplit; first done.
+  by rewrite later_equivI.
 Qed.
 
 Lemma ownI_open i P : wsat ∗ ownI i P ∗ ownE {[i]} ⊢ wsat ∗ ▷ P ∗ ownD {[i]}.
@@ -159,12 +152,10 @@ Proof.
       as (i & [? HIi%not_elem_of_dom]%not_elem_of_union & ?); eauto. }
   iDestruct "HE" as (X) "[Hi HE]"; iDestruct "Hi" as %(i & -> & HIi & ?).
   iMod (own_update with "Hw") as "[Hw HiP]".
-  { eapply auth_update_alloc,
-     (alloc_singleton_local_update _ i (invariant_unfold P)); last done.
-    by rewrite /= lookup_fmap HIi. }
+  { eapply (gmap_auth_ro_alloc _ i). by rewrite /= lookup_fmap HIi. }
   iModIntro; iExists i;  iSplit; [done|]. rewrite /ownI; iFrame "HiP".
   iExists (<[i:=P]>I); iSplitL "Hw".
-  { by rewrite fmap_insert insert_singleton_op ?lookup_fmap ?HIi. }
+  { by rewrite fmap_insert. }
   iApply (big_sepM_insert _ I); first done.
   iFrame "HI". iLeft. by rewrite /ownD; iFrame.
 Qed.
@@ -181,13 +172,11 @@ Proof.
       as (i & [? HIi%not_elem_of_dom]%not_elem_of_union & ?); eauto. }
   iDestruct "HD" as (X) "[Hi HD]"; iDestruct "Hi" as %(i & -> & HIi & ?).
   iMod (own_update with "Hw") as "[Hw HiP]".
-  { eapply auth_update_alloc,
-     (alloc_singleton_local_update _ i (invariant_unfold P)); last done.
-    by rewrite /= lookup_fmap HIi. }
+  { eapply (gmap_auth_ro_alloc _ i). by rewrite /= lookup_fmap HIi. }
   iModIntro; iExists i;  iSplit; [done|]. rewrite /ownI; iFrame "HiP".
   rewrite -/(ownD _). iFrame "HD".
   iIntros "HE". iExists (<[i:=P]>I); iSplitL "Hw".
-  { by rewrite fmap_insert insert_singleton_op ?lookup_fmap ?HIi. }
+  { by rewrite fmap_insert. }
   iApply (big_sepM_insert _ I); first done.
   iFrame "HI". by iRight.
 Qed.
@@ -197,8 +186,8 @@ End wsat.
 Lemma wsat_alloc `{!invPreG Σ} : ⊢ |==> ∃ _ : invG Σ, wsat ∗ ownE ⊤.
 Proof.
   iIntros.
-  iMod (own_alloc (● (∅ : gmap positive _))) as (γI) "HI";
-    first by rewrite auth_auth_valid.
+  iMod (own_alloc (gmap_auth_auth_ro ∅)) as (γI) "HI";
+    first by apply gmap_auth_auth_ro_valid.
   iMod (own_alloc (CoPset ⊤)) as (γE) "HE"; first done.
   iMod (own_alloc (GSet ∅)) as (γD) "HD"; first done.
   iModIntro; iExists (WsatG _ _ _ _ γI γE γD).
